Uncommitted minor changes

ft_tests/Timeout.bpl
@@ -21,9 +21,9 @@ var AT#intlst: List int;
 
 function AT#Min(x:int, y: int): int { if x <= y then x else y }
 
-// -- Types and global variables ---------------------------------
-type SeqType = <a>[Chan a][int]int;
-var Seq: SeqType;
+// -- Sequence numbering for FT ----------------------------------
+var SqnCh: <a>[Chan a][int]int;
+var SqnAct: [Actor]int;
 
 // ---------------------------------------------------------------
 // -- End of prelude ---------------------------------------------
@@ -31,7 +31,7 @@ var Seq: SeqType;
 
 axiom Base#L == 1;
 procedure Rep#anon$0#0()
-  modifies C, R, M, St;
+  modifies C, R, M, St, SqnCh, SqnAct;
 {
   var in: Chan (int);
   var out: Chan (int);
@@ -39,7 +39,7 @@ procedure Rep#anon$0#0()
   assume true;
 }
 procedure Split#anon$1#1()
-  modifies C, R, M, St;
+  modifies C, R, M, St, SqnCh, SqnAct;
 {
   var in: Chan (int);
   var out1: Chan (int);
@@ -48,7 +48,7 @@ procedure Split#anon$1#1()
   assume true;
 }
 procedure Adjudicator#normal#2()
-  modifies C, R, M, St;
+  modifies C, R, M, St, SqnCh, SqnAct;
 {
   var x1: Chan (int);
   var x2: Chan (int);
@@ -60,7 +60,7 @@ procedure Adjudicator#normal#2()
   assume true;
 }
 procedure Adjudicator#timeout#3()
-  modifies C, R, M, St;
+  modifies C, R, M, St, SqnCh, SqnAct;
 {
   var x1: Chan (int);
   var x2: Chan (int);
@@ -71,7 +71,7 @@ procedure Adjudicator#timeout#3()
   assume true;
 }
 procedure Adjudicator#readoff#4()
-  modifies C, R, M, St;
+  modifies C, R, M, St, SqnCh, SqnAct;
 {
   var x1: Chan (int);
   var x2: Chan (int);
@@ -83,7 +83,7 @@ procedure Adjudicator#readoff#4()
   assume true;
 }
 procedure Net#init#5()
-  modifies C, R, M, St;
+  modifies C, R, M, St, SqnCh, SqnAct;
 {
   assume C[Net#a] == 0;
   assume R[Net#a] == 0;
@@ -114,11 +114,15 @@ const unique Net#e: Chan (int);
 const unique Net#f: Chan (int);
 const unique Net#g: Chan (int);
 procedure Net#anon$2#entry#6()
-  modifies C, R, M, St;
+  modifies C, R, M, St, SqnCh, SqnAct;
 {
   var ActionPH#y1: int;
   var ActionPH#y2: int;
   var ActionPH#y3: int;
+  assume SqnAct[Net#spl] == 0;
+  assume SqnAct[Net#pri] == 0;
+  assume SqnAct[Net#sec] == 0;
+  assume SqnAct[Net#adj] == 0;
   assume L[Net#a] == (3 * Base#L);
   assume R[Net#a] == 0;
   assume C[Net#a] == 0;
@@ -170,18 +174,21 @@ procedure Net#anon$2#entry#6()
   assert {:msg "  Channel invariant might not hold on action entry (#24)"} (forall idx$: int :: 
     (0 <= idx$) && (idx$ < (R[Net#e] + C[Net#e])) ==> (M[Net#e][idx$] == M[Net#c][idx$])
   );
-  assert {:msg "  40.3: Channel invariant might not hold on action entry (#25)"} (R[Net#a] + C[Net#a]) <= 3;
-  assert {:msg "  47.3: Channel invariant might not hold on action entry (#26)"} C[Net#f] == 1;
-  assert {:msg "  48.3: Channel invariant might not hold on action entry (#27)"} C[Net#g] == R[Net#e];
-  assert {:msg "  49.3: Channel invariant might not hold on action entry (#28)"} R[Net#e] == M[Net#f][R[Net#f]];
-  assert {:msg "  50.3: Channel invariant might not hold on action entry (#29)"} R[Net#d] <= R[Net#e];
-  assert {:msg "  51.3: Channel invariant might not hold on action entry (#30)"} (0 < R[Net#d]) && (0 < R[Net#e]) ==> (M[Net#d][R[Net#d] - 1] <= M[Net#e][R[Net#e] - 1]);
-  assert {:msg "  52.3: Channel invariant might not hold on action entry (#31)"} (forall i: int :: 
+  assert {:msg "  Channel invariant might not hold on action entry (#25)"} (forall idx$: int :: 
+    (0 <= idx$) && (idx$ < (R[Net#a] + C[Net#a])) ==> (SqnCh[Net#a][idx$] == idx$)
+  );
+  assert {:msg "  40.3: Channel invariant might not hold on action entry (#26)"} (R[Net#a] + C[Net#a]) <= 3;
+  assert {:msg "  47.3: Channel invariant might not hold on action entry (#27)"} C[Net#f] == 1;
+  assert {:msg "  48.3: Channel invariant might not hold on action entry (#28)"} C[Net#g] == R[Net#e];
+  assert {:msg "  49.3: Channel invariant might not hold on action entry (#29)"} R[Net#e] == M[Net#f][R[Net#f]];
+  assert {:msg "  50.3: Channel invariant might not hold on action entry (#30)"} R[Net#d] <= R[Net#e];
+  assert {:msg "  51.3: Channel invariant might not hold on action entry (#31)"} (0 < R[Net#d]) && (0 < R[Net#e]) ==> (M[Net#d][R[Net#d] - 1] <= M[Net#e][R[Net#e] - 1]);
+  assert {:msg "  52.3: Channel invariant might not hold on action entry (#32)"} (forall i: int :: 
     (0 <= i) && (i < R[Net#e]) ==> (M[Net#g][i] == M[Net#e][i])
   );
 }
 procedure Net#anon$2#Split#anon$1#7()
-  modifies C, R, M, St;
+  modifies C, R, M, St, SqnCh, SqnAct;
 {
   var ActionPH#y1: int;
   var ActionPH#y2: int;
@@ -221,6 +228,9 @@ procedure Net#anon$2#Split#anon$1#7()
   );
   assume (forall idx$: int :: 
     (0 <= idx$) && (idx$ < (R[Net#e] + C[Net#e])) ==> (M[Net#e][idx$] == M[Net#c][idx$])
+  );
+  assume (forall idx$: int :: 
+    (0 <= idx$) && (idx$ < (R[Net#a] + C[Net#a])) ==> (SqnCh[Net#a][idx$] == idx$)
   );
   assume (R[Net#a] + C[Net#a]) <= 3;
   assume C[Net#f] == 1;
@@ -237,9 +247,12 @@ procedure Net#anon$2#Split#anon$1#7()
   R[Net#a] := R[Net#a] + 1;
   C[Net#a] := C[Net#a] - 1;
   M[Net#b][R[Net#b] + C[Net#b]] := in#i;
+  SqnCh[Net#b][R[Net#b] + C[Net#b]] := SqnAct[Net#spl];
   C[Net#b] := C[Net#b] + 1;
   M[Net#c][R[Net#c] + C[Net#c]] := in#i;
+  SqnCh[Net#c][R[Net#c] + C[Net#c]] := SqnAct[Net#spl];
   C[Net#c] := C[Net#c] + 1;
+  SqnAct[Net#spl] := SqnAct[Net#spl] + 1;
   assume 0 <= R[Net#a];
   assume 0 <= C[Net#a];
   assume (R[Net#a] + C[Net#a]) <= L[Net#a];
@@ -256,35 +269,38 @@ procedure Net#anon$2#Split#anon$1#7()
   assume 0 <= R[Net#g];
   assume 0 <= C[Net#g];
   assume R[Net#g] == 0;
-  assert {:msg "  Action at 8.3 ('anon$1') for actor instance 'spl' might not preserve the channel invariant (#48)"} (M[Net#a][0] == 0) && (M[Net#a][1] == 1) && (M[Net#a][2] == 2);
-  assert {:msg "  Action at 8.3 ('anon$1') for actor instance 'spl' might not preserve the channel invariant (#49)"} R[Net#a] == (R[Net#b] + C[Net#b]);
-  assert {:msg "  Action at 8.3 ('anon$1') for actor instance 'spl' might not preserve the channel invariant (#50)"} R[Net#a] == (R[Net#c] + C[Net#c]);
-  assert {:msg "  Action at 8.3 ('anon$1') for actor instance 'spl' might not preserve the channel invariant (#51)"} R[Net#b] == (R[Net#d] + C[Net#d]);
-  assert {:msg "  Action at 8.3 ('anon$1') for actor instance 'spl' might not preserve the channel invariant (#52)"} R[Net#c] == (R[Net#e] + C[Net#e]);
-  assert {:msg "  Action at 8.3 ('anon$1') for actor instance 'spl' might not preserve the channel invariant (#53)"} (forall idx$: int :: 
+  assert {:msg "  Action at 8.3 ('anon$1') for actor instance 'spl' might not preserve the channel invariant (#49)"} (M[Net#a][0] == 0) && (M[Net#a][1] == 1) && (M[Net#a][2] == 2);
+  assert {:msg "  Action at 8.3 ('anon$1') for actor instance 'spl' might not preserve the channel invariant (#50)"} R[Net#a] == (R[Net#b] + C[Net#b]);
+  assert {:msg "  Action at 8.3 ('anon$1') for actor instance 'spl' might not preserve the channel invariant (#51)"} R[Net#a] == (R[Net#c] + C[Net#c]);
+  assert {:msg "  Action at 8.3 ('anon$1') for actor instance 'spl' might not preserve the channel invariant (#52)"} R[Net#b] == (R[Net#d] + C[Net#d]);
+  assert {:msg "  Action at 8.3 ('anon$1') for actor instance 'spl' might not preserve the channel invariant (#53)"} R[Net#c] == (R[Net#e] + C[Net#e]);
+  assert {:msg "  Action at 8.3 ('anon$1') for actor instance 'spl' might not preserve the channel invariant (#54)"} (forall idx$: int :: 
     (0 <= idx$) && (idx$ < (R[Net#b] + C[Net#b])) ==> (M[Net#b][idx$] == M[Net#a][idx$])
   );
-  assert {:msg "  Action at 8.3 ('anon$1') for actor instance 'spl' might not preserve the channel invariant (#54)"} (forall idx$: int :: 
+  assert {:msg "  Action at 8.3 ('anon$1') for actor instance 'spl' might not preserve the channel invariant (#55)"} (forall idx$: int :: 
     (0 <= idx$) && (idx$ < (R[Net#c] + C[Net#c])) ==> (M[Net#c][idx$] == M[Net#a][idx$])
   );
-  assert {:msg "  Action at 8.3 ('anon$1') for actor instance 'spl' might not preserve the channel invariant (#55)"} (forall idx$: int :: 
+  assert {:msg "  Action at 8.3 ('anon$1') for actor instance 'spl' might not preserve the channel invariant (#56)"} (forall idx$: int :: 
     (0 <= idx$) && (idx$ < (R[Net#d] + C[Net#d])) ==> (M[Net#d][idx$] == M[Net#b][idx$])
   );
-  assert {:msg "  Action at 8.3 ('anon$1') for actor instance 'spl' might not preserve the channel invariant (#56)"} (forall idx$: int :: 
+  assert {:msg "  Action at 8.3 ('anon$1') for actor instance 'spl' might not preserve the channel invariant (#57)"} (forall idx$: int :: 
     (0 <= idx$) && (idx$ < (R[Net#e] + C[Net#e])) ==> (M[Net#e][idx$] == M[Net#c][idx$])
   );
-  assert {:msg "  40.3: Action at 8.3 ('anon$1') for actor instance 'spl' might not preserve the channel invariant (#57)"} (R[Net#a] + C[Net#a]) <= 3;
-  assert {:msg "  47.3: Action at 8.3 ('anon$1') for actor instance 'spl' might not preserve the channel invariant (#58)"} C[Net#f] == 1;
-  assert {:msg "  48.3: Action at 8.3 ('anon$1') for actor instance 'spl' might not preserve the channel invariant (#59)"} C[Net#g] == R[Net#e];
-  assert {:msg "  49.3: Action at 8.3 ('anon$1') for actor instance 'spl' might not preserve the channel invariant (#60)"} R[Net#e] == M[Net#f][R[Net#f]];
-  assert {:msg "  50.3: Action at 8.3 ('anon$1') for actor instance 'spl' might not preserve the channel invariant (#61)"} R[Net#d] <= R[Net#e];
-  assert {:msg "  51.3: Action at 8.3 ('anon$1') for actor instance 'spl' might not preserve the channel invariant (#62)"} (0 < R[Net#d]) && (0 < R[Net#e]) ==> (M[Net#d][R[Net#d] - 1] <= M[Net#e][R[Net#e] - 1]);
-  assert {:msg "  52.3: Action at 8.3 ('anon$1') for actor instance 'spl' might not preserve the channel invariant (#63)"} (forall i: int :: 
+  assert {:msg "  Action at 8.3 ('anon$1') for actor instance 'spl' might not preserve the channel invariant (#58)"} (forall idx$: int :: 
+    (0 <= idx$) && (idx$ < (R[Net#a] + C[Net#a])) ==> (SqnCh[Net#a][idx$] == idx$)
+  );
+  assert {:msg "  40.3: Action at 8.3 ('anon$1') for actor instance 'spl' might not preserve the channel invariant (#59)"} (R[Net#a] + C[Net#a]) <= 3;
+  assert {:msg "  47.3: Action at 8.3 ('anon$1') for actor instance 'spl' might not preserve the channel invariant (#60)"} C[Net#f] == 1;
+  assert {:msg "  48.3: Action at 8.3 ('anon$1') for actor instance 'spl' might not preserve the channel invariant (#61)"} C[Net#g] == R[Net#e];
+  assert {:msg "  49.3: Action at 8.3 ('anon$1') for actor instance 'spl' might not preserve the channel invariant (#62)"} R[Net#e] == M[Net#f][R[Net#f]];
+  assert {:msg "  50.3: Action at 8.3 ('anon$1') for actor instance 'spl' might not preserve the channel invariant (#63)"} R[Net#d] <= R[Net#e];
+  assert {:msg "  51.3: Action at 8.3 ('anon$1') for actor instance 'spl' might not preserve the channel invariant (#64)"} (0 < R[Net#d]) && (0 < R[Net#e]) ==> (M[Net#d][R[Net#d] - 1] <= M[Net#e][R[Net#e] - 1]);
+  assert {:msg "  52.3: Action at 8.3 ('anon$1') for actor instance 'spl' might not preserve the channel invariant (#65)"} (forall i: int :: 
     (0 <= i) && (i < R[Net#e]) ==> (M[Net#g][i] == M[Net#e][i])
   );
 }
 procedure Net#anon$2#Rep#anon$0#8()
-  modifies C, R, M, St;
+  modifies C, R, M, St, SqnCh, SqnAct;
 {
   var ActionPH#y1: int;
   var ActionPH#y2: int;
@@ -324,6 +340,9 @@ procedure Net#anon$2#Rep#anon$0#8()
   );
   assume (forall idx$: int :: 
     (0 <= idx$) && (idx$ < (R[Net#e] + C[Net#e])) ==> (M[Net#e][idx$] == M[Net#c][idx$])
+  );
+  assume (forall idx$: int :: 
+    (0 <= idx$) && (idx$ < (R[Net#a] + C[Net#a])) ==> (SqnCh[Net#a][idx$] == idx$)
   );
   assume (R[Net#a] + C[Net#a]) <= 3;
   assume C[Net#f] == 1;
@@ -340,7 +359,9 @@ procedure Net#anon$2#Rep#anon$0#8()
   R[Net#b] := R[Net#b] + 1;
   C[Net#b] := C[Net#b] - 1;
   M[Net#d][R[Net#d] + C[Net#d]] := in#i;
+  SqnCh[Net#d][R[Net#d] + C[Net#d]] := SqnAct[Net#pri];
   C[Net#d] := C[Net#d] + 1;
+  SqnAct[Net#pri] := SqnAct[Net#pri] + 1;
   assume 0 <= R[Net#a];
   assume 0 <= C[Net#a];
   assume (R[Net#a] + C[Net#a]) <= L[Net#a];
@@ -357,35 +378,38 @@ procedure Net#anon$2#Rep#anon$0#8()
   assume 0 <= R[Net#g];
   assume 0 <= C[Net#g];
   assume R[Net#g] == 0;
-  assert {:msg "  Action at 3.3 ('anon$0') for actor instance 'pri' might not preserve the channel invariant (#80)"} (M[Net#a][0] == 0) && (M[Net#a][1] == 1) && (M[Net#a][2] == 2);
-  assert {:msg "  Action at 3.3 ('anon$0') for actor instance 'pri' might not preserve the channel invariant (#81)"} R[Net#a] == (R[Net#b] + C[Net#b]);
-  assert {:msg "  Action at 3.3 ('anon$0') for actor instance 'pri' might not preserve the channel invariant (#82)"} R[Net#a] == (R[Net#c] + C[Net#c]);
-  assert {:msg "  Action at 3.3 ('anon$0') for actor instance 'pri' might not preserve the channel invariant (#83)"} R[Net#b] == (R[Net#d] + C[Net#d]);
-  assert {:msg "  Action at 3.3 ('anon$0') for actor instance 'pri' might not preserve the channel invariant (#84)"} R[Net#c] == (R[Net#e] + C[Net#e]);
-  assert {:msg "  Action at 3.3 ('anon$0') for actor instance 'pri' might not preserve the channel invariant (#85)"} (forall idx$: int :: 
+  assert {:msg "  Action at 3.3 ('anon$0') for actor instance 'pri' might not preserve the channel invariant (#82)"} (M[Net#a][0] == 0) && (M[Net#a][1] == 1) && (M[Net#a][2] == 2);
+  assert {:msg "  Action at 3.3 ('anon$0') for actor instance 'pri' might not preserve the channel invariant (#83)"} R[Net#a] == (R[Net#b] + C[Net#b]);
+  assert {:msg "  Action at 3.3 ('anon$0') for actor instance 'pri' might not preserve the channel invariant (#84)"} R[Net#a] == (R[Net#c] + C[Net#c]);
+  assert {:msg "  Action at 3.3 ('anon$0') for actor instance 'pri' might not preserve the channel invariant (#85)"} R[Net#b] == (R[Net#d] + C[Net#d]);
+  assert {:msg "  Action at 3.3 ('anon$0') for actor instance 'pri' might not preserve the channel invariant (#86)"} R[Net#c] == (R[Net#e] + C[Net#e]);
+  assert {:msg "  Action at 3.3 ('anon$0') for actor instance 'pri' might not preserve the channel invariant (#87)"} (forall idx$: int :: 
     (0 <= idx$) && (idx$ < (R[Net#b] + C[Net#b])) ==> (M[Net#b][idx$] == M[Net#a][idx$])
   );
-  assert {:msg "  Action at 3.3 ('anon$0') for actor instance 'pri' might not preserve the channel invariant (#86)"} (forall idx$: int :: 
+  assert {:msg "  Action at 3.3 ('anon$0') for actor instance 'pri' might not preserve the channel invariant (#88)"} (forall idx$: int :: 
     (0 <= idx$) && (idx$ < (R[Net#c] + C[Net#c])) ==> (M[Net#c][idx$] == M[Net#a][idx$])
   );
-  assert {:msg "  Action at 3.3 ('anon$0') for actor instance 'pri' might not preserve the channel invariant (#87)"} (forall idx$: int :: 
+  assert {:msg "  Action at 3.3 ('anon$0') for actor instance 'pri' might not preserve the channel invariant (#89)"} (forall idx$: int :: 
     (0 <= idx$) && (idx$ < (R[Net#d] + C[Net#d])) ==> (M[Net#d][idx$] == M[Net#b][idx$])
   );
-  assert {:msg "  Action at 3.3 ('anon$0') for actor instance 'pri' might not preserve the channel invariant (#88)"} (forall idx$: int :: 
+  assert {:msg "  Action at 3.3 ('anon$0') for actor instance 'pri' might not preserve the channel invariant (#90)"} (forall idx$: int :: 
     (0 <= idx$) && (idx$ < (R[Net#e] + C[Net#e])) ==> (M[Net#e][idx$] == M[Net#c][idx$])
   );
-  assert {:msg "  40.3: Action at 3.3 ('anon$0') for actor instance 'pri' might not preserve the channel invariant (#89)"} (R[Net#a] + C[Net#a]) <= 3;
-  assert {:msg "  47.3: Action at 3.3 ('anon$0') for actor instance 'pri' might not preserve the channel invariant (#90)"} C[Net#f] == 1;
-  assert {:msg "  48.3: Action at 3.3 ('anon$0') for actor instance 'pri' might not preserve the channel invariant (#91)"} C[Net#g] == R[Net#e];
-  assert {:msg "  49.3: Action at 3.3 ('anon$0') for actor instance 'pri' might not preserve the channel invariant (#92)"} R[Net#e] == M[Net#f][R[Net#f]];
-  assert {:msg "  50.3: Action at 3.3 ('anon$0') for actor instance 'pri' might not preserve the channel invariant (#93)"} R[Net#d] <= R[Net#e];
-  assert {:msg "  51.3: Action at 3.3 ('anon$0') for actor instance 'pri' might not preserve the channel invariant (#94)"} (0 < R[Net#d]) && (0 < R[Net#e]) ==> (M[Net#d][R[Net#d] - 1] <= M[Net#e][R[Net#e] - 1]);
-  assert {:msg "  52.3: Action at 3.3 ('anon$0') for actor instance 'pri' might not preserve the channel invariant (#95)"} (forall i: int :: 
+  assert {:msg "  Action at 3.3 ('anon$0') for actor instance 'pri' might not preserve the channel invariant (#91)"} (forall idx$: int :: 
+    (0 <= idx$) && (idx$ < (R[Net#a] + C[Net#a])) ==> (SqnCh[Net#a][idx$] == idx$)
+  );
+  assert {:msg "  40.3: Action at 3.3 ('anon$0') for actor instance 'pri' might not preserve the channel invariant (#92)"} (R[Net#a] + C[Net#a]) <= 3;
+  assert {:msg "  47.3: Action at 3.3 ('anon$0') for actor instance 'pri' might not preserve the channel invariant (#93)"} C[Net#f] == 1;
+  assert {:msg "  48.3: Action at 3.3 ('anon$0') for actor instance 'pri' might not preserve the channel invariant (#94)"} C[Net#g] == R[Net#e];
+  assert {:msg "  49.3: Action at 3.3 ('anon$0') for actor instance 'pri' might not preserve the channel invariant (#95)"} R[Net#e] == M[Net#f][R[Net#f]];
+  assert {:msg "  50.3: Action at 3.3 ('anon$0') for actor instance 'pri' might not preserve the channel invariant (#96)"} R[Net#d] <= R[Net#e];
+  assert {:msg "  51.3: Action at 3.3 ('anon$0') for actor instance 'pri' might not preserve the channel invariant (#97)"} (0 < R[Net#d]) && (0 < R[Net#e]) ==> (M[Net#d][R[Net#d] - 1] <= M[Net#e][R[Net#e] - 1]);
+  assert {:msg "  52.3: Action at 3.3 ('anon$0') for actor instance 'pri' might not preserve the channel invariant (#98)"} (forall i: int :: 
     (0 <= i) && (i < R[Net#e]) ==> (M[Net#g][i] == M[Net#e][i])
   );
 }
 procedure Net#anon$2#Rep#anon$0#9()
-  modifies C, R, M, St;
+  modifies C, R, M, St, SqnCh, SqnAct;
 {
   var ActionPH#y1: int;
   var ActionPH#y2: int;
@@ -426,6 +450,9 @@ procedure Net#anon$2#Rep#anon$0#9()
   assume (forall idx$: int :: 
     (0 <= idx$) && (idx$ < (R[Net#e] + C[Net#e])) ==> (M[Net#e][idx$] == M[Net#c][idx$])
   );
+  assume (forall idx$: int :: 
+    (0 <= idx$) && (idx$ < (R[Net#a] + C[Net#a])) ==> (SqnCh[Net#a][idx$] == idx$)
+  );
   assume (R[Net#a] + C[Net#a]) <= 3;
   assume C[Net#f] == 1;
   assume C[Net#g] == R[Net#e];
@@ -441,7 +468,9 @@ procedure Net#anon$2#Rep#anon$0#9()
   R[Net#c] := R[Net#c] + 1;
   C[Net#c] := C[Net#c] - 1;
   M[Net#e][R[Net#e] + C[Net#e]] := in#i;
+  SqnCh[Net#e][R[Net#e] + C[Net#e]] := SqnAct[Net#sec];
   C[Net#e] := C[Net#e] + 1;
+  SqnAct[Net#sec] := SqnAct[Net#sec] + 1;
   assume 0 <= R[Net#a];
   assume 0 <= C[Net#a];
   assume (R[Net#a] + C[Net#a]) <= L[Net#a];
@@ -458,35 +487,38 @@ procedure Net#anon$2#Rep#anon$0#9()
   assume 0 <= R[Net#g];
   assume 0 <= C[Net#g];
   assume R[Net#g] == 0;
-  assert {:msg "  Action at 3.3 ('anon$0') for actor instance 'sec' might not preserve the channel invariant (#112)"} (M[Net#a][0] == 0) && (M[Net#a][1] == 1) && (M[Net#a][2] == 2);
-  assert {:msg "  Action at 3.3 ('anon$0') for actor instance 'sec' might not preserve the channel invariant (#113)"} R[Net#a] == (R[Net#b] + C[Net#b]);
-  assert {:msg "  Action at 3.3 ('anon$0') for actor instance 'sec' might not preserve the channel invariant (#114)"} R[Net#a] == (R[Net#c] + C[Net#c]);
-  assert {:msg "  Action at 3.3 ('anon$0') for actor instance 'sec' might not preserve the channel invariant (#115)"} R[Net#b] == (R[Net#d] + C[Net#d]);
-  assert {:msg "  Action at 3.3 ('anon$0') for actor instance 'sec' might not preserve the channel invariant (#116)"} R[Net#c] == (R[Net#e] + C[Net#e]);
-  assert {:msg "  Action at 3.3 ('anon$0') for actor instance 'sec' might not preserve the channel invariant (#117)"} (forall idx$: int :: 
+  assert {:msg "  Action at 3.3 ('anon$0') for actor instance 'sec' might not preserve the channel invariant (#115)"} (M[Net#a][0] == 0) && (M[Net#a][1] == 1) && (M[Net#a][2] == 2);
+  assert {:msg "  Action at 3.3 ('anon$0') for actor instance 'sec' might not preserve the channel invariant (#116)"} R[Net#a] == (R[Net#b] + C[Net#b]);
+  assert {:msg "  Action at 3.3 ('anon$0') for actor instance 'sec' might not preserve the channel invariant (#117)"} R[Net#a] == (R[Net#c] + C[Net#c]);
+  assert {:msg "  Action at 3.3 ('anon$0') for actor instance 'sec' might not preserve the channel invariant (#118)"} R[Net#b] == (R[Net#d] + C[Net#d]);
+  assert {:msg "  Action at 3.3 ('anon$0') for actor instance 'sec' might not preserve the channel invariant (#119)"} R[Net#c] == (R[Net#e] + C[Net#e]);
+  assert {:msg "  Action at 3.3 ('anon$0') for actor instance 'sec' might not preserve the channel invariant (#120)"} (forall idx$: int :: 
     (0 <= idx$) && (idx$ < (R[Net#b] + C[Net#b])) ==> (M[Net#b][idx$] == M[Net#a][idx$])
   );
-  assert {:msg "  Action at 3.3 ('anon$0') for actor instance 'sec' might not preserve the channel invariant (#118)"} (forall idx$: int :: 
+  assert {:msg "  Action at 3.3 ('anon$0') for actor instance 'sec' might not preserve the channel invariant (#121)"} (forall idx$: int :: 
     (0 <= idx$) && (idx$ < (R[Net#c] + C[Net#c])) ==> (M[Net#c][idx$] == M[Net#a][idx$])
   );
-  assert {:msg "  Action at 3.3 ('anon$0') for actor instance 'sec' might not preserve the channel invariant (#119)"} (forall idx$: int :: 
+  assert {:msg "  Action at 3.3 ('anon$0') for actor instance 'sec' might not preserve the channel invariant (#122)"} (forall idx$: int :: 
     (0 <= idx$) && (idx$ < (R[Net#d] + C[Net#d])) ==> (M[Net#d][idx$] == M[Net#b][idx$])
   );
-  assert {:msg "  Action at 3.3 ('anon$0') for actor instance 'sec' might not preserve the channel invariant (#120)"} (forall idx$: int :: 
+  assert {:msg "  Action at 3.3 ('anon$0') for actor instance 'sec' might not preserve the channel invariant (#123)"} (forall idx$: int :: 
     (0 <= idx$) && (idx$ < (R[Net#e] + C[Net#e])) ==> (M[Net#e][idx$] == M[Net#c][idx$])
   );
-  assert {:msg "  40.3: Action at 3.3 ('anon$0') for actor instance 'sec' might not preserve the channel invariant (#121)"} (R[Net#a] + C[Net#a]) <= 3;
-  assert {:msg "  47.3: Action at 3.3 ('anon$0') for actor instance 'sec' might not preserve the channel invariant (#122)"} C[Net#f] == 1;
-  assert {:msg "  48.3: Action at 3.3 ('anon$0') for actor instance 'sec' might not preserve the channel invariant (#123)"} C[Net#g] == R[Net#e];
-  assert {:msg "  49.3: Action at 3.3 ('anon$0') for actor instance 'sec' might not preserve the channel invariant (#124)"} R[Net#e] == M[Net#f][R[Net#f]];
-  assert {:msg "  50.3: Action at 3.3 ('anon$0') for actor instance 'sec' might not preserve the channel invariant (#125)"} R[Net#d] <= R[Net#e];
-  assert {:msg "  51.3: Action at 3.3 ('anon$0') for actor instance 'sec' might not preserve the channel invariant (#126)"} (0 < R[Net#d]) && (0 < R[Net#e]) ==> (M[Net#d][R[Net#d] - 1] <= M[Net#e][R[Net#e] - 1]);
-  assert {:msg "  52.3: Action at 3.3 ('anon$0') for actor instance 'sec' might not preserve the channel invariant (#127)"} (forall i: int :: 
+  assert {:msg "  Action at 3.3 ('anon$0') for actor instance 'sec' might not preserve the channel invariant (#124)"} (forall idx$: int :: 
+    (0 <= idx$) && (idx$ < (R[Net#a] + C[Net#a])) ==> (SqnCh[Net#a][idx$] == idx$)
+  );
+  assert {:msg "  40.3: Action at 3.3 ('anon$0') for actor instance 'sec' might not preserve the channel invariant (#125)"} (R[Net#a] + C[Net#a]) <= 3;
+  assert {:msg "  47.3: Action at 3.3 ('anon$0') for actor instance 'sec' might not preserve the channel invariant (#126)"} C[Net#f] == 1;
+  assert {:msg "  48.3: Action at 3.3 ('anon$0') for actor instance 'sec' might not preserve the channel invariant (#127)"} C[Net#g] == R[Net#e];
+  assert {:msg "  49.3: Action at 3.3 ('anon$0') for actor instance 'sec' might not preserve the channel invariant (#128)"} R[Net#e] == M[Net#f][R[Net#f]];
+  assert {:msg "  50.3: Action at 3.3 ('anon$0') for actor instance 'sec' might not preserve the channel invariant (#129)"} R[Net#d] <= R[Net#e];
+  assert {:msg "  51.3: Action at 3.3 ('anon$0') for actor instance 'sec' might not preserve the channel invariant (#130)"} (0 < R[Net#d]) && (0 < R[Net#e]) ==> (M[Net#d][R[Net#d] - 1] <= M[Net#e][R[Net#e] - 1]);
+  assert {:msg "  52.3: Action at 3.3 ('anon$0') for actor instance 'sec' might not preserve the channel invariant (#131)"} (forall i: int :: 
     (0 <= i) && (i < R[Net#e]) ==> (M[Net#g][i] == M[Net#e][i])
   );
 }
 procedure Net#anon$2#Adjudicator#readoff#10()
-  modifies C, R, M, St;
+  modifies C, R, M, St, SqnCh, SqnAct;
 {
   var ActionPH#y1: int;
   var ActionPH#y2: int;
@@ -528,6 +560,9 @@ procedure Net#anon$2#Adjudicator#readoff#10()
   assume (forall idx$: int :: 
     (0 <= idx$) && (idx$ < (R[Net#e] + C[Net#e])) ==> (M[Net#e][idx$] == M[Net#c][idx$])
   );
+  assume (forall idx$: int :: 
+    (0 <= idx$) && (idx$ < (R[Net#a] + C[Net#a])) ==> (SqnCh[Net#a][idx$] == idx$)
+  );
   assume (R[Net#a] + C[Net#a]) <= 3;
   assume C[Net#f] == 1;
   assume C[Net#g] == R[Net#e];
@@ -547,7 +582,9 @@ procedure Net#anon$2#Adjudicator#readoff#10()
   R[Net#f] := R[Net#f] + 1;
   C[Net#f] := C[Net#f] - 1;
   M[Net#f][R[Net#f] + C[Net#f]] := c_in#c;
+  SqnCh[Net#f][R[Net#f] + C[Net#f]] := SqnAct[Net#adj];
   C[Net#f] := C[Net#f] + 1;
+  SqnAct[Net#adj] := SqnAct[Net#adj] + 1;
   assume 0 <= R[Net#a];
   assume 0 <= C[Net#a];
   assume (R[Net#a] + C[Net#a]) <= L[Net#a];
@@ -564,35 +601,38 @@ procedure Net#anon$2#Adjudicator#readoff#10()
   assume 0 <= R[Net#g];
   assume 0 <= C[Net#g];
   assume R[Net#g] == 0;
-  assert {:msg "  Action at 22.3 ('readoff') for actor instance 'adj' might not preserve the channel invariant (#144)"} (M[Net#a][0] == 0) && (M[Net#a][1] == 1) && (M[Net#a][2] == 2);
-  assert {:msg "  Action at 22.3 ('readoff') for actor instance 'adj' might not preserve the channel invariant (#145)"} R[Net#a] == (R[Net#b] + C[Net#b]);
-  assert {:msg "  Action at 22.3 ('readoff') for actor instance 'adj' might not preserve the channel invariant (#146)"} R[Net#a] == (R[Net#c] + C[Net#c]);
-  assert {:msg "  Action at 22.3 ('readoff') for actor instance 'adj' might not preserve the channel invariant (#147)"} R[Net#b] == (R[Net#d] + C[Net#d]);
-  assert {:msg "  Action at 22.3 ('readoff') for actor instance 'adj' might not preserve the channel invariant (#148)"} R[Net#c] == (R[Net#e] + C[Net#e]);
-  assert {:msg "  Action at 22.3 ('readoff') for actor instance 'adj' might not preserve the channel invariant (#149)"} (forall idx$: int :: 
+  assert {:msg "  Action at 22.3 ('readoff') for actor instance 'adj' might not preserve the channel invariant (#148)"} (M[Net#a][0] == 0) && (M[Net#a][1] == 1) && (M[Net#a][2] == 2);
+  assert {:msg "  Action at 22.3 ('readoff') for actor instance 'adj' might not preserve the channel invariant (#149)"} R[Net#a] == (R[Net#b] + C[Net#b]);
+  assert {:msg "  Action at 22.3 ('readoff') for actor instance 'adj' might not preserve the channel invariant (#150)"} R[Net#a] == (R[Net#c] + C[Net#c]);
+  assert {:msg "  Action at 22.3 ('readoff') for actor instance 'adj' might not preserve the channel invariant (#151)"} R[Net#b] == (R[Net#d] + C[Net#d]);
+  assert {:msg "  Action at 22.3 ('readoff') for actor instance 'adj' might not preserve the channel invariant (#152)"} R[Net#c] == (R[Net#e] + C[Net#e]);
+  assert {:msg "  Action at 22.3 ('readoff') for actor instance 'adj' might not preserve the channel invariant (#153)"} (forall idx$: int :: 
     (0 <= idx$) && (idx$ < (R[Net#b] + C[Net#b])) ==> (M[Net#b][idx$] == M[Net#a][idx$])
   );
-  assert {:msg "  Action at 22.3 ('readoff') for actor instance 'adj' might not preserve the channel invariant (#150)"} (forall idx$: int :: 
+  assert {:msg "  Action at 22.3 ('readoff') for actor instance 'adj' might not preserve the channel invariant (#154)"} (forall idx$: int :: 
     (0 <= idx$) && (idx$ < (R[Net#c] + C[Net#c])) ==> (M[Net#c][idx$] == M[Net#a][idx$])
   );
-  assert {:msg "  Action at 22.3 ('readoff') for actor instance 'adj' might not preserve the channel invariant (#151)"} (forall idx$: int :: 
+  assert {:msg "  Action at 22.3 ('readoff') for actor instance 'adj' might not preserve the channel invariant (#155)"} (forall idx$: int :: 
     (0 <= idx$) && (idx$ < (R[Net#d] + C[Net#d])) ==> (M[Net#d][idx$] == M[Net#b][idx$])
   );
-  assert {:msg "  Action at 22.3 ('readoff') for actor instance 'adj' might not preserve the channel invariant (#152)"} (forall idx$: int :: 
+  assert {:msg "  Action at 22.3 ('readoff') for actor instance 'adj' might not preserve the channel invariant (#156)"} (forall idx$: int :: 
     (0 <= idx$) && (idx$ < (R[Net#e] + C[Net#e])) ==> (M[Net#e][idx$] == M[Net#c][idx$])
   );
-  assert {:msg "  40.3: Action at 22.3 ('readoff') for actor instance 'adj' might not preserve the channel invariant (#153)"} (R[Net#a] + C[Net#a]) <= 3;
-  assert {:msg "  47.3: Action at 22.3 ('readoff') for actor instance 'adj' might not preserve the channel invariant (#154)"} C[Net#f] == 1;
-  assert {:msg "  48.3: Action at 22.3 ('readoff') for actor instance 'adj' might not preserve the channel invariant (#155)"} C[Net#g] == R[Net#e];
-  assert {:msg "  49.3: Action at 22.3 ('readoff') for actor instance 'adj' might not preserve the channel invariant (#156)"} R[Net#e] == M[Net#f][R[Net#f]];
-  assert {:msg "  50.3: Action at 22.3 ('readoff') for actor instance 'adj' might not preserve the channel invariant (#157)"} R[Net#d] <= R[Net#e];
-  assert {:msg "  51.3: Action at 22.3 ('readoff') for actor instance 'adj' might not preserve the channel invariant (#158)"} (0 < R[Net#d]) && (0 < R[Net#e]) ==> (M[Net#d][R[Net#d] - 1] <= M[Net#e][R[Net#e] - 1]);
-  assert {:msg "  52.3: Action at 22.3 ('readoff') for actor instance 'adj' might not preserve the channel invariant (#159)"} (forall i: int :: 
+  assert {:msg "  Action at 22.3 ('readoff') for actor instance 'adj' might not preserve the channel invariant (#157)"} (forall idx$: int :: 
+    (0 <= idx$) && (idx$ < (R[Net#a] + C[Net#a])) ==> (SqnCh[Net#a][idx$] == idx$)
+  );
+  assert {:msg "  40.3: Action at 22.3 ('readoff') for actor instance 'adj' might not preserve the channel invariant (#158)"} (R[Net#a] + C[Net#a]) <= 3;
+  assert {:msg "  47.3: Action at 22.3 ('readoff') for actor instance 'adj' might not preserve the channel invariant (#159)"} C[Net#f] == 1;
+  assert {:msg "  48.3: Action at 22.3 ('readoff') for actor instance 'adj' might not preserve the channel invariant (#160)"} C[Net#g] == R[Net#e];
+  assert {:msg "  49.3: Action at 22.3 ('readoff') for actor instance 'adj' might not preserve the channel invariant (#161)"} R[Net#e] == M[Net#f][R[Net#f]];
+  assert {:msg "  50.3: Action at 22.3 ('readoff') for actor instance 'adj' might not preserve the channel invariant (#162)"} R[Net#d] <= R[Net#e];
+  assert {:msg "  51.3: Action at 22.3 ('readoff') for actor instance 'adj' might not preserve the channel invariant (#163)"} (0 < R[Net#d]) && (0 < R[Net#e]) ==> (M[Net#d][R[Net#d] - 1] <= M[Net#e][R[Net#e] - 1]);
+  assert {:msg "  52.3: Action at 22.3 ('readoff') for actor instance 'adj' might not preserve the channel invariant (#164)"} (forall i: int :: 
     (0 <= i) && (i < R[Net#e]) ==> (M[Net#g][i] == M[Net#e][i])
   );
 }
 procedure Net#anon$2#Adjudicator#normal#11()
-  modifies C, R, M, St;
+  modifies C, R, M, St, SqnCh, SqnAct;
 {
   var ActionPH#y1: int;
   var ActionPH#y2: int;
@@ -634,6 +674,9 @@ procedure Net#anon$2#Adjudicator#normal#11()
   );
   assume (forall idx$: int :: 
     (0 <= idx$) && (idx$ < (R[Net#e] + C[Net#e])) ==> (M[Net#e][idx$] == M[Net#c][idx$])
+  );
+  assume (forall idx$: int :: 
+    (0 <= idx$) && (idx$ < (R[Net#a] + C[Net#a])) ==> (SqnCh[Net#a][idx$] == idx$)
   );
   assume (R[Net#a] + C[Net#a]) <= 3;
   assume C[Net#f] == 1;
@@ -657,9 +700,12 @@ procedure Net#anon$2#Adjudicator#normal#11()
   R[Net#f] := R[Net#f] + 1;
   C[Net#f] := C[Net#f] - 1;
   M[Net#g][R[Net#g] + C[Net#g]] := x1#i;
+  SqnCh[Net#g][R[Net#g] + C[Net#g]] := SqnAct[Net#adj];
   C[Net#g] := C[Net#g] + 1;
   M[Net#f][R[Net#f] + C[Net#f]] := c_in#c + 1;
+  SqnCh[Net#f][R[Net#f] + C[Net#f]] := SqnAct[Net#adj];
   C[Net#f] := C[Net#f] + 1;
+  SqnAct[Net#adj] := SqnAct[Net#adj] + 1;
   assume 0 <= R[Net#a];
   assume 0 <= C[Net#a];
   assume (R[Net#a] + C[Net#a]) <= L[Net#a];
@@ -676,35 +722,38 @@ procedure Net#anon$2#Adjudicator#normal#11()
   assume 0 <= R[Net#g];
   assume 0 <= C[Net#g];
   assume R[Net#g] == 0;
-  assert {:msg "  Action at 14.3 ('normal') for actor instance 'adj' might not preserve the channel invariant (#176)"} (M[Net#a][0] == 0) && (M[Net#a][1] == 1) && (M[Net#a][2] == 2);
-  assert {:msg "  Action at 14.3 ('normal') for actor instance 'adj' might not preserve the channel invariant (#177)"} R[Net#a] == (R[Net#b] + C[Net#b]);
-  assert {:msg "  Action at 14.3 ('normal') for actor instance 'adj' might not preserve the channel invariant (#178)"} R[Net#a] == (R[Net#c] + C[Net#c]);
-  assert {:msg "  Action at 14.3 ('normal') for actor instance 'adj' might not preserve the channel invariant (#179)"} R[Net#b] == (R[Net#d] + C[Net#d]);
-  assert {:msg "  Action at 14.3 ('normal') for actor instance 'adj' might not preserve the channel invariant (#180)"} R[Net#c] == (R[Net#e] + C[Net#e]);
-  assert {:msg "  Action at 14.3 ('normal') for actor instance 'adj' might not preserve the channel invariant (#181)"} (forall idx$: int :: 
+  assert {:msg "  Action at 14.3 ('normal') for actor instance 'adj' might not preserve the channel invariant (#181)"} (M[Net#a][0] == 0) && (M[Net#a][1] == 1) && (M[Net#a][2] == 2);
+  assert {:msg "  Action at 14.3 ('normal') for actor instance 'adj' might not preserve the channel invariant (#182)"} R[Net#a] == (R[Net#b] + C[Net#b]);
+  assert {:msg "  Action at 14.3 ('normal') for actor instance 'adj' might not preserve the channel invariant (#183)"} R[Net#a] == (R[Net#c] + C[Net#c]);
+  assert {:msg "  Action at 14.3 ('normal') for actor instance 'adj' might not preserve the channel invariant (#184)"} R[Net#b] == (R[Net#d] + C[Net#d]);
+  assert {:msg "  Action at 14.3 ('normal') for actor instance 'adj' might not preserve the channel invariant (#185)"} R[Net#c] == (R[Net#e] + C[Net#e]);
+  assert {:msg "  Action at 14.3 ('normal') for actor instance 'adj' might not preserve the channel invariant (#186)"} (forall idx$: int :: 
     (0 <= idx$) && (idx$ < (R[Net#b] + C[Net#b])) ==> (M[Net#b][idx$] == M[Net#a][idx$])
   );
-  assert {:msg "  Action at 14.3 ('normal') for actor instance 'adj' might not preserve the channel invariant (#182)"} (forall idx$: int :: 
+  assert {:msg "  Action at 14.3 ('normal') for actor instance 'adj' might not preserve the channel invariant (#187)"} (forall idx$: int :: 
     (0 <= idx$) && (idx$ < (R[Net#c] + C[Net#c])) ==> (M[Net#c][idx$] == M[Net#a][idx$])
   );
-  assert {:msg "  Action at 14.3 ('normal') for actor instance 'adj' might not preserve the channel invariant (#183)"} (forall idx$: int :: 
+  assert {:msg "  Action at 14.3 ('normal') for actor instance 'adj' might not preserve the channel invariant (#188)"} (forall idx$: int :: 
     (0 <= idx$) && (idx$ < (R[Net#d] + C[Net#d])) ==> (M[Net#d][idx$] == M[Net#b][idx$])
   );
-  assert {:msg "  Action at 14.3 ('normal') for actor instance 'adj' might not preserve the channel invariant (#184)"} (forall idx$: int :: 
+  assert {:msg "  Action at 14.3 ('normal') for actor instance 'adj' might not preserve the channel invariant (#189)"} (forall idx$: int :: 
     (0 <= idx$) && (idx$ < (R[Net#e] + C[Net#e])) ==> (M[Net#e][idx$] == M[Net#c][idx$])
   );
-  assert {:msg "  40.3: Action at 14.3 ('normal') for actor instance 'adj' might not preserve the channel invariant (#185)"} (R[Net#a] + C[Net#a]) <= 3;
-  assert {:msg "  47.3: Action at 14.3 ('normal') for actor instance 'adj' might not preserve the channel invariant (#186)"} C[Net#f] == 1;
-  assert {:msg "  48.3: Action at 14.3 ('normal') for actor instance 'adj' might not preserve the channel invariant (#187)"} C[Net#g] == R[Net#e];
-  assert {:msg "  49.3: Action at 14.3 ('normal') for actor instance 'adj' might not preserve the channel invariant (#188)"} R[Net#e] == M[Net#f][R[Net#f]];
-  assert {:msg "  50.3: Action at 14.3 ('normal') for actor instance 'adj' might not preserve the channel invariant (#189)"} R[Net#d] <= R[Net#e];
-  assert {:msg "  51.3: Action at 14.3 ('normal') for actor instance 'adj' might not preserve the channel invariant (#190)"} (0 < R[Net#d]) && (0 < R[Net#e]) ==> (M[Net#d][R[Net#d] - 1] <= M[Net#e][R[Net#e] - 1]);
-  assert {:msg "  52.3: Action at 14.3 ('normal') for actor instance 'adj' might not preserve the channel invariant (#191)"} (forall i: int :: 
+  assert {:msg "  Action at 14.3 ('normal') for actor instance 'adj' might not preserve the channel invariant (#190)"} (forall idx$: int :: 
+    (0 <= idx$) && (idx$ < (R[Net#a] + C[Net#a])) ==> (SqnCh[Net#a][idx$] == idx$)
+  );
+  assert {:msg "  40.3: Action at 14.3 ('normal') for actor instance 'adj' might not preserve the channel invariant (#191)"} (R[Net#a] + C[Net#a]) <= 3;
+  assert {:msg "  47.3: Action at 14.3 ('normal') for actor instance 'adj' might not preserve the channel invariant (#192)"} C[Net#f] == 1;
+  assert {:msg "  48.3: Action at 14.3 ('normal') for actor instance 'adj' might not preserve the channel invariant (#193)"} C[Net#g] == R[Net#e];
+  assert {:msg "  49.3: Action at 14.3 ('normal') for actor instance 'adj' might not preserve the channel invariant (#194)"} R[Net#e] == M[Net#f][R[Net#f]];
+  assert {:msg "  50.3: Action at 14.3 ('normal') for actor instance 'adj' might not preserve the channel invariant (#195)"} R[Net#d] <= R[Net#e];
+  assert {:msg "  51.3: Action at 14.3 ('normal') for actor instance 'adj' might not preserve the channel invariant (#196)"} (0 < R[Net#d]) && (0 < R[Net#e]) ==> (M[Net#d][R[Net#d] - 1] <= M[Net#e][R[Net#e] - 1]);
+  assert {:msg "  52.3: Action at 14.3 ('normal') for actor instance 'adj' might not preserve the channel invariant (#197)"} (forall i: int :: 
     (0 <= i) && (i < R[Net#e]) ==> (M[Net#g][i] == M[Net#e][i])
   );
 }
 procedure Net#anon$2#Adjudicator#timeout#12()
-  modifies C, R, M, St;
+  modifies C, R, M, St, SqnCh, SqnAct;
 {
   var ActionPH#y1: int;
   var ActionPH#y2: int;
@@ -746,6 +795,9 @@ procedure Net#anon$2#Adjudicator#timeout#12()
   assume (forall idx$: int :: 
     (0 <= idx$) && (idx$ < (R[Net#e] + C[Net#e])) ==> (M[Net#e][idx$] == M[Net#c][idx$])
   );
+  assume (forall idx$: int :: 
+    (0 <= idx$) && (idx$ < (R[Net#a] + C[Net#a])) ==> (SqnCh[Net#a][idx$] == idx$)
+  );
   assume (R[Net#a] + C[Net#a]) <= 3;
   assume C[Net#f] == 1;
   assume C[Net#g] == R[Net#e];
@@ -764,9 +816,12 @@ procedure Net#anon$2#Adjudicator#timeout#12()
   R[Net#f] := R[Net#f] + 1;
   C[Net#f] := C[Net#f] - 1;
   M[Net#g][R[Net#g] + C[Net#g]] := x2#j;
+  SqnCh[Net#g][R[Net#g] + C[Net#g]] := SqnAct[Net#adj];
   C[Net#g] := C[Net#g] + 1;
   M[Net#f][R[Net#f] + C[Net#f]] := c_in#c + 1;
+  SqnCh[Net#f][R[Net#f] + C[Net#f]] := SqnAct[Net#adj];
   C[Net#f] := C[Net#f] + 1;
+  SqnAct[Net#adj] := SqnAct[Net#adj] + 1;
   assume 0 <= R[Net#a];
   assume 0 <= C[Net#a];
   assume (R[Net#a] + C[Net#a]) <= L[Net#a];
@@ -783,35 +838,38 @@ procedure Net#anon$2#Adjudicator#timeout#12()
   assume 0 <= R[Net#g];
   assume 0 <= C[Net#g];
   assume R[Net#g] == 0;
-  assert {:msg "  Action at 18.3 ('timeout') for actor instance 'adj' might not preserve the channel invariant (#208)"} (M[Net#a][0] == 0) && (M[Net#a][1] == 1) && (M[Net#a][2] == 2);
-  assert {:msg "  Action at 18.3 ('timeout') for actor instance 'adj' might not preserve the channel invariant (#209)"} R[Net#a] == (R[Net#b] + C[Net#b]);
-  assert {:msg "  Action at 18.3 ('timeout') for actor instance 'adj' might not preserve the channel invariant (#210)"} R[Net#a] == (R[Net#c] + C[Net#c]);
-  assert {:msg "  Action at 18.3 ('timeout') for actor instance 'adj' might not preserve the channel invariant (#211)"} R[Net#b] == (R[Net#d] + C[Net#d]);
-  assert {:msg "  Action at 18.3 ('timeout') for actor instance 'adj' might not preserve the channel invariant (#212)"} R[Net#c] == (R[Net#e] + C[Net#e]);
-  assert {:msg "  Action at 18.3 ('timeout') for actor instance 'adj' might not preserve the channel invariant (#213)"} (forall idx$: int :: 
+  assert {:msg "  Action at 18.3 ('timeout') for actor instance 'adj' might not preserve the channel invariant (#214)"} (M[Net#a][0] == 0) && (M[Net#a][1] == 1) && (M[Net#a][2] == 2);
+  assert {:msg "  Action at 18.3 ('timeout') for actor instance 'adj' might not preserve the channel invariant (#215)"} R[Net#a] == (R[Net#b] + C[Net#b]);
+  assert {:msg "  Action at 18.3 ('timeout') for actor instance 'adj' might not preserve the channel invariant (#216)"} R[Net#a] == (R[Net#c] + C[Net#c]);
+  assert {:msg "  Action at 18.3 ('timeout') for actor instance 'adj' might not preserve the channel invariant (#217)"} R[Net#b] == (R[Net#d] + C[Net#d]);
+  assert {:msg "  Action at 18.3 ('timeout') for actor instance 'adj' might not preserve the channel invariant (#218)"} R[Net#c] == (R[Net#e] + C[Net#e]);
+  assert {:msg "  Action at 18.3 ('timeout') for actor instance 'adj' might not preserve the channel invariant (#219)"} (forall idx$: int :: 
     (0 <= idx$) && (idx$ < (R[Net#b] + C[Net#b])) ==> (M[Net#b][idx$] == M[Net#a][idx$])
   );
-  assert {:msg "  Action at 18.3 ('timeout') for actor instance 'adj' might not preserve the channel invariant (#214)"} (forall idx$: int :: 
+  assert {:msg "  Action at 18.3 ('timeout') for actor instance 'adj' might not preserve the channel invariant (#220)"} (forall idx$: int :: 
     (0 <= idx$) && (idx$ < (R[Net#c] + C[Net#c])) ==> (M[Net#c][idx$] == M[Net#a][idx$])
   );
-  assert {:msg "  Action at 18.3 ('timeout') for actor instance 'adj' might not preserve the channel invariant (#215)"} (forall idx$: int :: 
+  assert {:msg "  Action at 18.3 ('timeout') for actor instance 'adj' might not preserve the channel invariant (#221)"} (forall idx$: int :: 
     (0 <= idx$) && (idx$ < (R[Net#d] + C[Net#d])) ==> (M[Net#d][idx$] == M[Net#b][idx$])
   );
-  assert {:msg "  Action at 18.3 ('timeout') for actor instance 'adj' might not preserve the channel invariant (#216)"} (forall idx$: int :: 
+  assert {:msg "  Action at 18.3 ('timeout') for actor instance 'adj' might not preserve the channel invariant (#222)"} (forall idx$: int :: 
     (0 <= idx$) && (idx$ < (R[Net#e] + C[Net#e])) ==> (M[Net#e][idx$] == M[Net#c][idx$])
   );
-  assert {:msg "  40.3: Action at 18.3 ('timeout') for actor instance 'adj' might not preserve the channel invariant (#217)"} (R[Net#a] + C[Net#a]) <= 3;
-  assert {:msg "  47.3: Action at 18.3 ('timeout') for actor instance 'adj' might not preserve the channel invariant (#218)"} C[Net#f] == 1;
-  assert {:msg "  48.3: Action at 18.3 ('timeout') for actor instance 'adj' might not preserve the channel invariant (#219)"} C[Net#g] == R[Net#e];
-  assert {:msg "  49.3: Action at 18.3 ('timeout') for actor instance 'adj' might not preserve the channel invariant (#220)"} R[Net#e] == M[Net#f][R[Net#f]];
-  assert {:msg "  50.3: Action at 18.3 ('timeout') for actor instance 'adj' might not preserve the channel invariant (#221)"} R[Net#d] <= R[Net#e];
-  assert {:msg "  51.3: Action at 18.3 ('timeout') for actor instance 'adj' might not preserve the channel invariant (#222)"} (0 < R[Net#d]) && (0 < R[Net#e]) ==> (M[Net#d][R[Net#d] - 1] <= M[Net#e][R[Net#e] - 1]);
-  assert {:msg "  52.3: Action at 18.3 ('timeout') for actor instance 'adj' might not preserve the channel invariant (#223)"} (forall i: int :: 
+  assert {:msg "  Action at 18.3 ('timeout') for actor instance 'adj' might not preserve the channel invariant (#223)"} (forall idx$: int :: 
+    (0 <= idx$) && (idx$ < (R[Net#a] + C[Net#a])) ==> (SqnCh[Net#a][idx$] == idx$)
+  );
+  assert {:msg "  40.3: Action at 18.3 ('timeout') for actor instance 'adj' might not preserve the channel invariant (#224)"} (R[Net#a] + C[Net#a]) <= 3;
+  assert {:msg "  47.3: Action at 18.3 ('timeout') for actor instance 'adj' might not preserve the channel invariant (#225)"} C[Net#f] == 1;
+  assert {:msg "  48.3: Action at 18.3 ('timeout') for actor instance 'adj' might not preserve the channel invariant (#226)"} C[Net#g] == R[Net#e];
+  assert {:msg "  49.3: Action at 18.3 ('timeout') for actor instance 'adj' might not preserve the channel invariant (#227)"} R[Net#e] == M[Net#f][R[Net#f]];
+  assert {:msg "  50.3: Action at 18.3 ('timeout') for actor instance 'adj' might not preserve the channel invariant (#228)"} R[Net#d] <= R[Net#e];
+  assert {:msg "  51.3: Action at 18.3 ('timeout') for actor instance 'adj' might not preserve the channel invariant (#229)"} (0 < R[Net#d]) && (0 < R[Net#e]) ==> (M[Net#d][R[Net#d] - 1] <= M[Net#e][R[Net#e] - 1]);
+  assert {:msg "  52.3: Action at 18.3 ('timeout') for actor instance 'adj' might not preserve the channel invariant (#230)"} (forall i: int :: 
     (0 <= i) && (i < R[Net#e]) ==> (M[Net#g][i] == M[Net#e][i])
   );
 }
 procedure Net#anon$2#exit#13()
-  modifies C, R, M, St;
+  modifies C, R, M, St, SqnCh, SqnAct;
 {
   var ActionPH#y1: int;
   var ActionPH#y2: int;
@@ -849,6 +907,9 @@ procedure Net#anon$2#exit#13()
   );
   assume (forall idx$: int :: 
     (0 <= idx$) && (idx$ < (R[Net#e] + C[Net#e])) ==> (M[Net#e][idx$] == M[Net#c][idx$])
+  );
+  assume (forall idx$: int :: 
+    (0 <= idx$) && (idx$ < (R[Net#a] + C[Net#a])) ==> (SqnCh[Net#a][idx$] == idx$)
   );
   assume (R[Net#a] + C[Net#a]) <= 3;
   assume C[Net#f] == 1;
